theory/CoreRel/Equiv.v
@@ -59,14 +59,16 @@ Section Equiv.
     with signature align_eqv ==> align_eqv ==> align_eqv
       as ACSeq_eqv_cong.
   Proof.
-    intros r1 r1' r1_eqv c2 c2' c2_eqv ((st1, st2), (st1', st2')); simpl; split;
-      intros; In_inversion; simpl in *; In_intro.
-    - apply r1_eqv; eauto.
-    - apply c2_eqv; eauto.
-    - apply r1_eqv; eauto.
-    - apply c2_eqv; eauto.
+   intros r1 r1' r1_eqv c2 c2' c2_eqv ((st1, st2), (st1', st2')). simpl. split.
+   intros. In_inversion. simpl in *. eexists _,_,_,_. split. eapply r1_eqv.
+   eassumption. split. eapply c2_eqv. eassumption. inversion H1; subst.
+   inversion H2; subst. auto.
+   intros. In_inversion. simpl in *. eexists _,_,_,_. split. 
+   eapply r1_eqv. eassumption. split.
+   apply c2_eqv. eassumption. inversion H1; subst. inversion H2; subst.
+   auto.
   Qed.
-
+    
   #[global]
   Add Parametric Morphism : ACIf
     with signature bexp_eqv ==> bexp_eqv ==> align_eqv ==> align_eqv ==> align_eqv
@@ -104,8 +106,10 @@ Section Equiv.
           apply while_body_monotone.
           firstorder.
         * apply LFP_fold.
-          apply while_body_monotone.
-          firstorder.
+          apply while_body_monotone. simpl in *. right. right.
+          split. apply b1_eqv. assumption. split. apply b2_eqv.
+          assumption. eexists _,_,_,_. split. apply r1_eqv.
+          eassumption. split. eassumption. firstorder.
     - eapply Ind in H.
       + apply H.
       + unfold FClosed.
@@ -119,142 +123,260 @@ Section Equiv.
           apply while_body_monotone.
           firstorder.
         * apply LFP_fold.
-          apply while_body_monotone.
-          firstorder.
+          apply while_body_monotone. simpl in *. right. right.
+          split. apply b1_eqv. assumption. split. apply b2_eqv.
+          assumption. eexists _,_,_,_. split. apply r1_eqv. 
+          eassumption. split. eassumption. firstorder.
   Qed.
 
   (* More interestingly, we can prove analogues of algebraic
-     equivalences from the BiKAT paper: *)
+     equivalences from the BiKAT paper: - Prove from here*)
 
   Lemma rel_def : forall s1 s2,
       <{ <|s1 | s2|> }> ==R <{ <| s1 | skip|>;; <|skip | s2 |> }>.
   Proof.
-    intros s1 s2 ((st1, st2), (st1', st2')); firstorder;
-      simpl in *; In_inversion;
-      firstorder.
-  Qed.
-
-  Lemma rel_comm : forall s1 s2,
+   intros s1 s2 ((st1, st2), (st1', st2')); firstorder;
+   simpl in *; In_inversion; subst. firstorder.
+   (*Normal, Normal*)
+   eexists _,_,_,_. split. eexists _,_. split. eassumption.
+   split. firstorder. eauto. split. eexists _,_. split. 
+   firstorder. split. eassumption. eauto. auto. 
+   eexists _,_. split. eassumption. split. rewrite <- H6 in H8.
+   inversion H8; subst. eassumption. rewrite H0 in H7.
+   rewrite H7 in H4. auto.
+ Qed.
+   
+ Lemma rel_comm : forall s1 s2,
       <{ <| skip | s2 |>;; <|s1 | skip |> }> ==R <{ <| s1 | skip|>;; <|skip | s2 |> }>.
-  Proof.
-    intros s1 s2 ((st1, st2), (st1', st2')); firstorder;
-      simpl in *; In_inversion;
-      firstorder.
-  Qed.
+ Proof.
+   intros s1 s2 ((st1, st2), (st1', st2')); firstorder;
+   simpl in *; In_inversion; firstorder. 
+   (*Normal, Normal*)
+   eexists _,_,_,_. split. eexists _,_. split. rewrite <- H7 in H.
+   inversion H; subst. eassumption. firstorder. 
+   split. eexists _,_. firstorder. eassumption. rewrite H8 in H3.
+   rewrite <- H3 in H5. auto.
+   (*Normal, Normal*)
+   eexists _,_,_,_. split. eexists _,_. split. firstorder.
+   split. rewrite <- H6 in H8. inversion H8; subst. eassumption. eauto.
+   (*Normal, Normal*)
+   split. eexists _,_. split. eassumption. firstorder. 
+   rewrite <- H0 in H4. rewrite <- H4 in H7. auto.
+ Qed.
 
   Lemma prod_hom_l : forall s1 s2,
       <{ <|s1; s2 | skip|> }> ==R <{ <| s1 | skip|>;; <|s2 | skip |> }>.
   Proof.
     intros s1 s2 ((st1, st2), (st1', st2')); firstorder;
-      simpl in *; In_inversion;
-      firstorder.
-  Qed.
+    simpl in *; In_inversion; firstorder. 
+    eexists _,_,_,_. split. eexists _,_. firstorder. eassumption.
+    split. eexists _,_. firstorder. eassumption. auto.
+    eexists _,_. split. left. eexists. split. eassumption.
+    inversion H7; subst. eassumption.
+    firstorder. rewrite <- H5 in H3. rewrite H3 in H8. 
+    rewrite <- H8 in H6. symmetry. assumption.
+  Qed.    
 
   Lemma prod_hom_r : forall s1 s2,
       <{ <| skip | s1; s2|> }> ==R <{ <| skip | s1 |>;; <|skip | s2 |> }>.
   Proof.
     intros s1 s2 ((st1, st2), (st1', st2')); firstorder;
-      simpl in *; In_inversion;
-      firstorder.
+    simpl in *; In_inversion; firstorder.
+    eexists _,_,_,_. split. eexists _,_. firstorder. eassumption.
+    split. eexists _,_. firstorder. eassumption. auto.
+    eexists _,_. firstorder. left. eexists. split. 
+    eassumption. inversion H5; subst. inversion H8; subst.
+    assumption. rewrite <- H0 in H4. rewrite <- H7 in H.
+    rewrite <- H in H4. assumption.   
   Qed.
 
   Lemma prod_seq_assoc : forall r1 r2 r3,
       <{ (r1 ;; r2);; r3  }> ==R <{ r1;; r2;; r3 }>.
   Proof.
     intros r1 r2 r3 ((st1, st2), (st1', st2')); firstorder;
-      simpl in *; In_inversion; In_intro; eauto; firstorder.
+    simpl in *; In_inversion; firstorder. 
+    eexists _,_,_,_. split. eassumption. split. 
+    eexists _,_,_,_. firstorder. eassumption. inversion H4; subst.
+    inversion H5; subst. eassumption. auto.
+    eexists _,_,_,_. split. eexists _,_,_,_. firstorder. 
+    eassumption. eassumption. firstorder. eassumption. 
+    rewrite H4 in H1. assumption. rewrite H5 in H2. assumption.
   Qed.
 
+(*problem*)
   Lemma if_align : forall b1 b2 c1 c2 c3 c4,
       <{ <| if b1 then c1 else c2 end | if b2 then c3 else c4 end |> }>
       ==R <{ifR <|b1 | b2|> then <|c1 | c3|> else ifR <|b1 | BNot b2|> then <|c1 | c4|>
             else ifR <|BNot b1 | b2|> then <|c2 | c3|> else <|c2 | c4|> end end end}> .
   Proof.
-    intros b1 b2 c1 c2 c3 c4 ((st1, st2), (st1', st2')). split.
-    intros. In_inversion. firstorder.
-    intros. simpl in H. In_inversion; firstorder. simpl in H,H0,H1,H2,H3.
-    apply bexp_eqv_unique with b1 false true st1 in H. discriminate H. assumption.
-    simpl in H, H0, H1, H2, H3. apply bexp_eqv_unique with b1 false true st1 in H.
-    discriminate H. assumption. simpl in H, H0, H1, H2, H3.
-    apply bexp_eqv_unique with b2 false true st2 in H. discriminate H.
-    assumption. simpl in H,H0,H1,H2,H3. apply bexp_eqv_unique with b2 false true st2 in H.
-    discriminate H. assumption.
-  Qed.
+   intros b1 b2 c1 c2 c3 c4 ((st1, st2), (st1', st2')); firstorder;
+   simpl in *; In_inversion; firstorder.
+   (*true, true*)
+   left. eexists _,_. firstorder. eexists _,_. firstorder.
+   eassumption. eassumption. assumption. assumption.
+   (*false true*)
+   right. left. eexists _,_. split. assumption. split. right.
+   left. eexists _,_. split. assumption. split. left.
+   eexists _,_. firstorder. eexists _,_. firstorder. 
+   eassumption. eassumption. eauto. auto.
+   (*true false*)
+   right. right. eexists _,_. firstorder. left. eexists _,_.
+   firstorder. eexists _,_. firstorder. eassumption. eassumption.
+   assumption. assumption.
+   (*false false*)
+   right. right. eexists _,_. split. assumption. split. right.
+   left. eexists _,_. split. assumption. split. right. right.
+   eexists _,_. firstorder. eexists _,_. firstorder. eassumption.
+   eassumption. eauto. auto.
+   (*true true*) 
+   eexists _,_. split. left. firstorder. eassumption.
+   split. left. firstorder. eassumption. rewrite H5 in H2.
+   rewrite H6 in H3. auto.
+   (*discriminate*)
+   apply bexp_eqv_unique with b1 false true st1 in H.
+   discriminate H. assumption.
+   (*false true*)
+   simpl in H3. eexists _,_. split. right. firstorder.
+   eassumption. split. left. firstorder. eassumption. 
+   rewrite H11 in H8. rewrite H8 in H4. rewrite H4 in H1.
+   rewrite H12 in H9. rewrite H9 in H5. rewrite H5 in H2. auto.
+   (*discriminate*)
+   simpl in H3. apply bexp_eqv_unique with b1 false true st1 in H.
+   discriminate H. assumption.
+   (*false false*)
+   eexists _,_. split. right. firstorder. eassumption. split.
+   right. firstorder. eassumption. rewrite H10 in H7.
+   rewrite H7 in H4. rewrite H4 in H1. rewrite H11 in H8.
+   rewrite H8 in H5. rewrite H5 in H2. auto.
+   (*false true*)
+   simpl in H0,H3. eexists _,_. split. right. firstorder.
+   eassumption. split. left. firstorder. eassumption. 
+   (*H11 -> H8 -> H4 -> H1*)
+   rewrite H11 in H8. rewrite H8 in H4. rewrite H4 in H1.
+   (*H12 -> H9 -> H5 -> H2*)
+   rewrite H12 in H9. rewrite H9 in H5. rewrite H5 in H2. auto.
+   (*discriminate*)
+   simpl in H0, H3. apply bexp_eqv_unique with b1 false true st1 in H.
+   discriminate H. assumption.
+   (*dicriminate*)
+   simpl in H0. apply bexp_eqv_unique with b2 true false st2 in H0.
+   discriminate H0. assumption.
+   (*true false*)
+   simpl in H3. eexists _,_. split. left. firstorder. eassumption.
+   split. right. firstorder. eassumption. 
+   (*H8 -> H5 -> H1*) rewrite H8 in H5. rewrite H5 in H1.
+   (*H9 -> H6 -> H2*) rewrite H9 in H6. rewrite H6 in H2. auto.
+   (*discriminate*)
+   simpl in *. apply bexp_eqv_unique with b2 false true st2 in H.
+   discriminate H. assumption.
+   (*discriminate*)
+   simpl in *. apply bexp_eqv_unique with b1 true false st1 in H3.
+   discriminate H3. assumption.
+   (*false false*)
+   eexists _,_. split. right. firstorder. eassumption. split.
+   right. firstorder. eassumption. 
+   (*H10 -> H7 -> H4 -> H1*) rewrite H10 in H7. rewrite H7 in H4.
+   rewrite H4 in H1.
+   (*H11 -> H8 -> H5 -> H2*) rewrite H11 in H8. rewrite H8 in H5.
+   rewrite H5 in H2. auto.
+   (*discriminate*)
+   simpl in *. apply bexp_eqv_unique with b2 true false st2 in H0.
+   discriminate H0. assumption. 
+   (*discriminate*)
+   simpl in *. apply bexp_eqv_unique with b2 true false st2 in H0.
+   discriminate H0. assumption. 
+   (*discriminate*)
+   simpl in *. apply bexp_eqv_unique with b2 true false st2 in H0.
+   discriminate H0. assumption.
+ Qed. 
 
-  Lemma whileR_false_L : forall b1 b2 r,
+   
+  (*From here*)
+ Lemma whileR_false_L : forall b1 b2 r,
       bexp_eqv b1 <{false}> ->
       <{ whileR <|b1 | b2|> do r end  }> ==R <{ <|skip|skip|> }> .
   Proof.
-    intros b1 b2 r b1_eqv ((st1, st2), (st1', st2')); split;
-      intros; In_inversion; firstorder;
-      apply Denotational_BigStep_Adequate in H.
-    - eapply BigStep_bexp_eqv with (st := st1) in b1_eqv.
-      inversion H; simpl in *; try congruence.
-    - eapply BigStep_bexp_eqv with (st := st1) in b1_eqv.
-      inversion H; simpl in *; try congruence.
+   
+    intros b1 b2 r b1_eqv ((st1, st2), (st1', st2')); 
+      simpl in *; split; intros; In_inversion. 
+      apply LFP_fold in H. In_inversion; subst.
+      (*b1 is false*)
+      simpl in *. eexists _,_. firstorder.
+      simpl in *. eexists _,_. firstorder.
+      simpl in *. apply b1_eqv in H. discriminate H.
+      apply while_body_monotone. apply LFP_unfold.
+      apply while_body_monotone. left. firstorder. 
+      inversion H; subst. inversion H0; subst. 
+      inversion H1; subst. inversion H2; subst. reflexivity.
+      inversion H2; subst. symmetry. assumption.
   Qed.
+
 
   Lemma whileR_false_R : forall b1 b2 r,
       bexp_eqv b2 <{false}> ->
       <{ whileR <|b1 | b2|> do r end  }> ==R <{ <|skip|skip|> }> .
   Proof.
-    intros b1 b2 r b2_eqv ((st1, st2), (st1', st2')); split;
-      intros; In_inversion; firstorder.
-    - simpl in H; apply LFP_fold in H; try apply while_body_monotone.
-      In_inversion.
-      + compute in H0, H1; subst; firstorder.
-      + compute in H0, H1; subst; firstorder.
-      + simpl in *.
-        apply b2_eqv in H0; compute in H0; discriminate.
-    - simpl in H; apply LFP_fold in H; try apply while_body_monotone.
-      In_inversion.
-      + compute in H0, H1; subst; firstorder.
-      + compute in H0, H1; subst; firstorder.
-      + simpl in *.
-        apply b2_eqv in H0; compute in H0; discriminate.
+      intros b1 b2 r b1_eqv ((st1, st2), (st1', st2')); 
+      simpl in *; split; intros; In_inversion. 
+      apply LFP_fold in H. In_inversion; subst.
+      (*b1 is false*)
+      simpl in *. eexists _,_. firstorder.
+      simpl in *. eexists _,_. firstorder.
+      simpl in *. apply b1_eqv in H0. discriminate H0.
+      apply while_body_monotone. apply LFP_unfold.
+      apply while_body_monotone. right. left. firstorder. 
+      inversion H; subst. inversion H0; subst.  
+      inversion H1; subst. inversion H2; subst. reflexivity.
+      inversion H2; subst. symmetry. assumption.
   Qed.
 
+ (*Normal -> Normal*)
   Lemma whileR_false_L' : forall b1 b2 r st1 st2,
       (denote_B b1) (false, st1) ->
-      [[<{ whileR <|b1 | b2|> do r end  }>]]R (st1, st2, (st1, st2)).
+      [[<{ whileR <|b1 | b2|> do r end  }>]]R (st1, st2, (RNormal st1, RNormal st2)).
   Proof.
     firstorder.
   Qed.
 
   Lemma whileR_false_R' : forall b1 b2 r st1 st2,
       (denote_B b2) (false, st2) ->
-      [[<{ whileR <|b1 | b2|> do r end  }>]]R (st1, st2, (st1, st2)).
+      [[<{ whileR <|b1 | b2|> do r end  }>]]R (st1, st2, (RNormal st1, RNormal st2)).
   Proof.
     firstorder.
   Qed.
 
   Lemma whileR_false_L'' : forall b1 b2 r st1 st2 st1' st2',
       (denote_B b1) (false, st1) ->
-      [[<{ whileR <|b1 | b2|> do r end  }>]]R (st1, st2, (st1', st2')) ->
+      [[<{ whileR <|b1 | b2|> do r end  }>]]R (st1, st2, (RNormal st1', RNormal st2')) ->
       st1 = st1' /\ st2 = st2'.
   Proof.
     simpl; intros.
     apply LFP_fold in H0; try apply while_body_monotone.
     In_inversion.
-    - compute in H0, H1; subst; firstorder.
-    - compute in H0, H1; subst; firstorder.
+    - compute in H0, H1; subst; firstorder. inversion H1; subst. reflexivity.
+      inversion H2. reflexivity.
+    - compute in H0, H1; subst; firstorder. inversion H1; subst. reflexivity.
+      inversion H2. reflexivity.
     - apply BigStep_B_Denotational_Adequate in H;
         apply BigStep_B_Denotational_Adequate in H0; simpl in *; congruence.
   Qed.
 
   Lemma whileR_false_R'' : forall b1 b2 r st1 st2 st1' st2',
       (denote_B b2) (false, st2) ->
-      [[<{ whileR <|b1 | b2|> do r end  }>]]R (st1, st2, (st1', st2')) ->
+      [[<{ whileR <|b1 | b2|> do r end  }>]]R (st1, st2, (RNormal st1', RNormal st2')) ->
       st1 = st1' /\ st2 = st2'.
   Proof.
     simpl; intros.
     apply LFP_fold in H0; try apply while_body_monotone.
     In_inversion.
-    - compute in H0, H1; subst; firstorder.
-    - compute in H0, H1; subst; firstorder.
-    - apply BigStep_B_Denotational_Adequate in H;
-        apply BigStep_B_Denotational_Adequate in H1; simpl in *; congruence.
-  Qed.
+    - compute in H0, H1; subst; firstorder. inversion H1; subst. reflexivity.
+      inversion H2. reflexivity.
+    - compute in H0, H1; subst; firstorder. inversion H1; subst. reflexivity.
+      inversion H2. reflexivity.
+    - simpl in *. apply BigStep_B_Denotational_Adequate in H.
+      apply BigStep_B_Denotational_Adequate in H1. rewrite H1 in H.
+      discriminate H.
+ Qed.
 
   Lemma whileR_unroll : forall b1 b2 r,
       <{ whileR <|b1 | b2|> do r end  }>
@@ -265,72 +387,123 @@ Section Equiv.
     apply LFP_fold in H; try apply while_body_monotone.
     In_inversion.
     - compute in H0, H1; subst; firstorder.
-      In_intro.
-      + firstorder.
-      + eapply whileR_false_L'; eauto.
-    - compute in H0, H1; subst; firstorder.
-      In_intro.
-      + firstorder.
-      + eapply whileR_false_R'; eauto.
-    - simpl in *; firstorder.
+      + firstorder. simpl in H. eapply whileR_false_L'. eauto.      
+        unfold FClosed.
+        intros ((stL, stR), (stL', stR')) ?.
+        In_inversion; subst.
+        simpl in *. eexists _,_,_,_. split. right. left.
+        eexists _,_. firstorder. eexists _,_. firstorder.
+        split. apply LFP_fold. apply while_body_monotone. 
+        left. firstorder. inversion H1; subst. inversion H2; subst.
+        simpl. auto. simpl in H0.
+        eexists _,_,_,_. split. right. right. eexists _,_.
+        firstorder. eassumption.  eexists _,_. firstorder.
+        split. apply LFP_unfold. apply while_body_monotone.
+        right. left. firstorder. inversion H1; subst. inversion H2; subst.
+        simpl. auto.
+        simpl in *. (*true, true*) eexists _,_,_,_. split. left. eexists _,_.
+        firstorder. eassumption. split. apply LFP_unfold. apply while_body_monotone.
+        (*true true*) right. right. firstorder. eexists _,_,_,_. split.
+        eassumption. split. inversion H11; subst. inversion H12; subst. eassumption.
+        eauto. inversion H4; subst. inversion H5; subst. auto.
+        simpl in *. (*true true*) 
+        apply LFP_fold in H6. In_inversion; subst. 
+        compute in H4,H5,H7,H8,H10,H11,H13,H14,H15,H16. simpl in H6.
+        eexists _,_,_,_. split. left. eexists _,_. firstorder. eassumption.
+        firstorder. rewrite H4. rewrite <- H9 in H13. rewrite H13 in H10.
+        rewrite H10 in H15. rewrite H15 in H7. assumption.
+        rewrite H5. rewrite <- H12 in H14. rewrite H14 in H11. rewrite H11 in H16.
+        rewrite H16 in H8. assumption.
+        simpl in H6. compute in H4,H5,H7,H8,H10,H11,H13,H14,H15,H16. eexists _,_,_,_.
+        split. left. eexists _,_. firstorder. eassumption. firstorder.
+        rewrite H4. rewrite <- H9 in H13. rewrite H13 in H10.
+        rewrite H10 in H15. rewrite H15 in H7. assumption. 
+        rewrite H5. rewrite <- H12 in H14. rewrite H14 in H11. rewrite H11 in H16.
+        rewrite H16 in H8. assumption.
+        simpl in *.
+        compute in  H4,H5,H7,H8,H10,H11,H13,H14, H18, H19. rewrite H13 in H10.
+        rewrite <- H9 in H10. inversion H10; subst. apply bexp_eqv_unique with b1 false true stL'' in H3.
+        discriminate H3. assumption. apply while_body_monotone.
+        simpl in H0,H1,H2,H3. compute in H4,H5,H7,H8,H10,H11,H13,H14.
+        eexists _,_,_,_. split. left. eexists _,_. firstorder. eassumption. split.
+        rewrite <- H9 in H13. rewrite H13 in H10. inversion H10; subst.
+        rewrite <- H12 in H14. rewrite H14 in H11. inversion H11; subst. eassumption.
+        rewrite H4. rewrite H5. auto.
+      - (*b2 is false*) simpl in H. compute in H0, H1. subst. eexists _,_,_,_. split. right.
+        right. eexists _,_. firstorder. eexists _,_. firstorder. split.
+        firstorder. auto.
+      - (*true, true*) simpl in H,H0,H1. compute in H3, H4. subst. eexists _,_,_,_.
+        split. left. eexists _,_. firstorder. eassumption. split. eassumption. auto.
+      - (*true, true*) compute in H1,H2,H5,H6. subst. apply LFP_fold. apply while_body_monotone.
+        right. right. firstorder. eexists _,_,_,_. split. eassumption. inversion H5; subst. 
+        inversion H6; subst. split. eassumption. auto.
+      - (*b1 is false*) compute in H1,H2,H4,H5,H7,H8. subst. rewrite <- H3 in H7.
+        rewrite H7 in H4. rewrite <- H6 in H8. rewrite H8 in H5. inversion H4; subst. inversion H5; subst.
+        assumption.
+     - (*b2 is false*) compute in H1,H2,H4,H5,H7,H8. subst. rewrite <- H3 in H7. rewrite H7 in H4.
+        rewrite <- H6 in H8. rewrite H8 in H5. inversion H4; subst. inversion H5; subst.
+        assumption.
   Qed.
+
 
   Lemma whileR_lockstep : forall b1 b2 s1 s2,
       <{ <| while b1 do s1 end | while b2 do s2 end |>  }>
       ==R <{whileR <|b1 | b2|> do <|s1 | s2|> end;;
           <| while b1 do s1 end | while b2 do s2 end |> }>.
   Proof.
-    intros b1 b2 s1 s2 ((st1, st2), (st1', st2')); split; intros X_In.
-    - eapply CR.Semantics.BigStep_Denotational_Sound.
-      eapply CR.Semantics.Denotational_BigStep_Adequate in X_In.
-      inversion X_In; subst; simpl in *; clear X_In.
-      remember <{ while b1 do s1 end}>.
-      revert st2 st2' s2 Heqc H5; induction H3; intros; subst;
-        intros; first [discriminate | injection Heqc; intros; subst; clear Heqc].
-      + econstructor.
-        * eapply E_ACWhileFalseL; simpl; eauto.
-        * econstructor; simpl; eauto.
-          apply E_WhileFalse; eauto.
-      + clear IHceval1.
-        inversion H5; subst; intros.
-        * econstructor.
-          -- eapply E_ACWhileFalseR; simpl; eauto.
-          -- econstructor; eauto.
-             eapply E_WhileTrue; eauto.
-        * eapply CR.Semantics.Denotational_BigStep_Adequate.
-          eapply ACSeq_eqv_cong.
-          eapply whileR_unroll.
-          reflexivity.
-          eapply prod_seq_assoc.
-          eapply CR.Semantics.BigStep_Denotational_Sound.
-          econstructor.
-          econstructor; eauto.
-          econstructor; eauto.
-          eapply IHceval2; eauto.
-    - eapply CR.Semantics.Denotational_BigStep_Adequate in X_In;
-        inversion X_In; subst; clear X_In.
-      remember <{whileR <| b1 | b2 |> do <| s1 | s2 |> end}> as r eqn:Heqr;
-        revert  st1' st2' Heqr H4; induction H1;
-        intros; first [discriminate | injection Heqr; intros; subst; clear Heqr].
-      + clear IHaceval1; specialize (IHaceval2 _ _ eq_refl H4).
-        eapply block_eqv_cong.
-        eapply If_while_eq.
-        eapply If_while_eq.
-        eapply CR.Semantics.BigStep_Denotational_Sound.
-        eapply CR.Semantics.Denotational_BigStep_Adequate in IHaceval2.
-        revert H H0 H1_ IHaceval2.
-        econstructor.
-        * econstructor; eauto.
-          inversion H1_; subst.
-          econstructor; eauto.
-          inversion IHaceval2; subst; intros; eauto.
-        * econstructor; eauto.
-          inversion H1_; subst.
-          econstructor; eauto.
-          inversion IHaceval2; subst; intros; eauto.
-      + eapply CR.Semantics.BigStep_Denotational_Sound; eauto.
-      + eapply CR.Semantics.BigStep_Denotational_Sound; eauto.
+    intros b1 b2 s1 s2 ((st1, st2), (st1', st2')); split; intros. inversion H; subst.
+    inversion H0; subst. destruct H1 as [H11 H12]. destruct H12 as [H121 H122].
+    destruct H122 as [? ?]. subst. 
+    (*bring it to form suitable for induction*)
+    eapply Imp.Semantics.Denotational_BigStep_Adequate in H11. 
+    eapply Imp.Semantics.Denotational_BigStep_Adequate in H121.
+    eapply CR.Semantics.BigStep_Denotational_Sound. clear H. clear H0.
+    remember <{ while b1 do s1 end}>. remember (RNormal x).  
+    generalize dependent st2. generalize dependent s2. generalize dependent b2.
+    induction H11. discriminate. discriminate. discriminate. discriminate.
+    discriminate. discriminate. injection Heqc; intros; subst; clear Heqc.
+    (*sequence: normal, normal*)
+    eapply E_ACSeqNormal. 
+    (*L - false*) eapply E_ACWhileFalseL; simpl; eauto.
+    (*<| s1 | s2 |> Normal*) eapply E_ACBlockNormal; simpl; eauto.
+    (*L - false Imp: Normal*) eapply E_WhileFalse; eauto. 
+    (*while*) intros. clear IHcevalr1. inversion H121; subst; intros.
+    econstructor. eapply E_ACWhileFalseR; simpl; eauto. 
+    econstructor; eauto. simpl. eapply E_WhileTrueNormal; eauto.
+    (*b2 is true*) injection Heqc; intros; subst; clear Heqc. 
+    eapply CR.Semantics.Denotational_BigStep_Adequate.
+    eapply ACSeq_eqv_cong. eapply whileR_unroll. reflexivity. eapply prod_seq_assoc.
+    eapply CR.Semantics.BigStep_Denotational_Sound. econstructor. econstructor; eauto.
+    econstructor; eauto. eapply IHcevalr2; eauto.
+    (*error - discriminate*) discriminate.
+    (*no match - discriminate*) discriminate.
+    (*error - discriminate*) discriminate.
+    (*OTHER SIDE*)
+    inversion H; subst. inversion H0; subst. inversion H1; subst. inversion H2; subst.
+    clear H0. clear H1. clear H2. clear H. destruct H3 as [? ?]. destruct H0 as [? ?].
+    destruct H1 as [? ?]. subst. eapply CR.Semantics.Denotational_BigStep_Adequate in H, H0.
+    remember <{whileR <| b1 | b2 |> do <| s1 | s2 |> end}> as r eqn:Heqr. 
+    remember (RNormal x, RNormal x0). generalize dependent x1. generalize dependent x2.
+    induction H. discriminate. discriminate. discriminate. discriminate. discriminate.
+    discriminate. discriminate. discriminate.
+    (*while - while*) injection Heqr; intros; subst; clear Heqr. 
+    clear IHaceval1. firstorder. eapply block_eqv_cong.
+    eapply If_while_eq. eapply If_while_eq. eapply CR.Semantics.BigStep_Denotational_Sound.
+    specialize H3 with x2 x1. apply H3 in H6. 
+    eapply CR.Semantics.Denotational_BigStep_Adequate in H6. 
+    econstructor; eauto. econstructor; eauto.
+    econstructor; eauto. inversion H1; subst. eassumption.
+    inversion H6; subst. eauto. econstructor; eauto.
+    econstructor; eauto. inversion H1; subst. eauto. inversion H6; subst; eauto.
+    (*Error, Normal*) discriminate.
+    (*while, Normal*) injection Heqr; subst; clear Heqr. injection Heqp; subst; clear Heqp.
+    intros. subst.  eapply CR.Semantics.BigStep_Denotational_Sound; eauto.
+    (*while, Normal*) injection Heqr; subst; clear Heqr. injection Heqp; subst; clear Heqp.
+    intros. subst.  eapply CR.Semantics.BigStep_Denotational_Sound; eauto.
+
   Qed.
+    
+
 
 End Equiv.
 
