theory/CoreRel/Semantics.v
@@ -25,51 +25,76 @@ Section Semantics.
   (* The operational semantics relate a pair of (disjoint) initial
    s tates to a pair of (disjoint) final state. *)
 
-  Definition state := @state M.
+  Definition state := @state M. 
+  Definition result := @result M. 
+
 
   Definition rel_state := (state * state)%type.
+  Definition rel_result := (result * result)%type.
 
-  Inductive aceval : algn_com -> rel_state -> rel_state -> Prop :=
-  | E_ACBlock : forall s1 s2 rst st1' st2',
-      fst rst =[ s1 ]=> st1' ->
-    snd rst =[ s2 ]=> st2' ->
-      rst =<[ <| s1 | s2 |> ]>=> (st1', st2')
+  (*If one errors -> both error*)
 
-| E_ACSeq : forall r1 r2 rst rst'' rst',
-    rst =<[ r1 ]>=> rst'' ->
-    rst'' =<[ r2 ]>=> rst' ->
+  Inductive aceval : algn_com -> rel_state -> rel_result -> Prop :=
+
+  | E_ACBlockNormal : forall s1 s2 rst st1' st2',
+      fst rst =[ s1 ]=> RNormal st1' ->
+      snd rst =[ s2 ]=> RNormal st2' ->
+      rst =<[ <| s1 | s2 |> ]>=> (RNormal st1', RNormal st2')
+
+  | E_ACBlockErrorP1 : forall s1 s2 rst,
+      fst rst =[ s1 ]=> RError ->
+      rst =<[ <| s1 | s2 |> ]>=> (RError, RError) (*add P2*)
+
+  | E_ACBlockErrorP2 : forall s1 s2 st rst,
+      fst rst =[ s1 ]=> RNormal st ->
+      snd rst =[ s2 ]=> RError ->
+      rst =<[ <| s1 | s2 |> ]>=> (RError, RError) 
+
+  | E_ACSeqNormal : forall r1 r2 rst st st' rst',
+    rst =<[ r1 ]>=> (RNormal st, RNormal st') ->
+    (st, st') =<[ r2 ]>=> rst' ->
     rst =<[ r1 ;; r2 ]>=> rst'
+ 
+  | E_ACSeqError : forall r1 r2 rst,
+    rst =<[ r1 ]>=> (RError, RError) ->
+    rst =<[ r1 ;; r2 ]>=> (RError, RError)
 
-| E_ACIfTrue : forall b1 b2 r1 r2 rst rst',
+  | E_ACIfTrue : forall b1 b2 r1 r2 rst rst',
     beval (fst rst) b1 = true ->
     beval (snd rst) b2 = true ->
     rst =<[ r1 ]>=> rst' ->
     rst =<[ ifR <| b1 | b2 |> then r1 else r2 end ]>=> rst'
 
-| E_ACIfFalseL : forall b1 b2 r1 r2 rst rst',
+  | E_ACIfFalseL : forall b1 b2 r1 r2 rst rst',
     beval (fst rst) b1 = false ->
     rst =<[ r2 ]>=> rst' ->
     rst =<[ ifR <| b1 | b2 |> then r1 else r2 end ]>=> rst'
 
-| E_ACIfFalseR : forall b1 b2 r1 r2 rst rst',
+  | E_ACIfFalseR : forall b1 b2 r1 r2 rst rst',
     beval (snd rst) b2 = false ->
     rst =<[ r2 ]>=> rst' ->
     rst =<[ ifR <| b1 | b2 |> then r1 else r2 end ]>=> rst'
 
-| E_ACWhileTrue : forall b1 b2 r rst rst' rst'',
+  | E_ACWhileTrueNormal : forall b1 b2 r rst st st' rst',
     beval (fst rst) b1 = true ->
     beval (snd rst) b2 = true ->
-    rst =<[ r ]>=> rst'' ->
-    rst'' =<[ whileR <| b1 | b2 |> do r end ]>=> rst' ->
+    rst =<[ r ]>=> (RNormal st, RNormal st') ->
+    (st, st') =<[ whileR <| b1 | b2 |> do r end ]>=> rst' ->
     rst =<[ whileR <| b1 | b2 |> do r end ]>=> rst'
 
-| E_ACWhileFalseL : forall b1 b2 r rst,
-    beval (fst rst) b1 = false ->
-    rst =<[ whileR <| b1 | b2 |> do r end ]>=> rst
+  | E_ACWhileTrueError : forall b1 b2 r rst,
+    beval (fst rst) b1 = true ->
+    beval (snd rst) b2 = true ->
+    rst =<[ r ]>=> (RError, RError) ->
+    rst =<[ whileR <| b1 | b2 |> do r end ]>=> (RError, RError)
 
-| E_ACWhileFalseR : forall b1 b2 r rst,
-    beval (snd rst) b2 = false ->
-    rst =<[ whileR <| b1 | b2 |> do r end ]>=> rst
+  | E_ACWhileFalseL : forall b1 b2 r st1 st2,
+    beval st1 b1 = false ->
+    (st1, st2) =<[ whileR <| b1 | b2 |> do r end ]>=> (RNormal st1, RNormal st2)
+
+  | E_ACWhileFalseR : forall b1 b2 r st1 st2,
+    beval st2 b2 = false ->
+    (st1, st2) =<[ whileR <| b1 | b2 |> do r end ]>=> (RNormal st1, RNormal st2)
 
 where "st =<[ r ]>=> st'" := (aceval r st st').
 
@@ -77,7 +102,7 @@ where "st =<[ r ]>=> st'" := (aceval r st st').
 (* The semantic domain for commands is pairs of initial and final
    relational states: *)
 
-Definition algn_com_dom := PSet (rel_state * rel_state)%type.
+Definition algn_com_dom := PSet (rel_state * rel_result)%type.
 
 (*⟦<s1 | s2> ⟧RC ≡ {( σL, σL', σR, σR') |
                       (σL, σL') ∈ ⟦s1⟧C ⋀ (σR, σR') ∈ ⟦s2⟧C  }
@@ -104,19 +129,30 @@ Definition algn_com_dom := PSet (rel_state * rel_state)%type.
                                       ⋀ (σL2, σL3, σR2, σR3) ∈ rec} *)
 
 (*The denotation of while loops uses the least fixed point [LFP]
-  combinator defined in Fixpoints.v. *)
+  combinator defined in Fixpoints.v. 
 
-Fixpoint denote_algn_com (r : algn_com) : algn_com_dom :=
+
+    <{c1; c2}> => {{ (st, st') |
+                   (exists st'',
+                   (st, RNormal st'') ∈ [[c1]] /\ (st'', st') ∈ [[c2]]) 
+                 \/ ((st, RError) ∈ [[c1]] /\ st' = RError)}}
+
+*)
+
+(*Fixpoint denote_algn_com (r : algn_com) : algn_com_dom :=
   match r with
   | <{ <| s1 | s2 |> }> =>
       {{ ((stL, stR), (stL', stR')) |
-         (stL, stL') ∈ denote_Com s1 /\ (stR, stR') ∈ denote_Com s2 }}
+         (exists st st', (stL, RNormal st) ∈ denote_Com s1 /\ (stR, RNormal st') ∈ denote_Com s2 
+          /\ stL' = RNormal st /\ stR' = RNormal st') \/ ((stL, RError) ∈ denote_Com s1 
+          /\ stL' = RError /\ stR' = RError) \/ (exists st, (stL, RNormal st) ∈ denote_Com s1 /\ 
+          (stR, RError) ∈ denote_Com s2  /\ stL' = RError /\ stR' = RError) }}
 
   | <{ r1;; r2 }> =>
       {{ ((stL, stR), (stL', stR')) |
-         exists stL'' stR'',
-         ((stL, stR), (stL'', stR'')) ∈ [[ r1 ]]R /\
-           ((stL'', stR''), (stL', stR')) ∈ [[r2]]R }}
+         (exists stL'' stR'',
+         ((stL, stR), (RNormal stL'', RNormal stR'')) ∈ [[ r1 ]]R /\
+           ((stL'', stR''), (stL', stR')) ∈ [[r2]]R ) \/ (((stL, stR), (RError, RError)) ∈ [[ r1 ]]R /\ stL' = RError /\ stR' = RError) }}
 
   | <{ ifR <| b1 | b2 |> then r1 else r2 end }> =>
       {{ ((stL, stR), (stL', stR')) |
@@ -131,15 +167,60 @@ Fixpoint denote_algn_com (r : algn_com) : algn_com_dom :=
   | <{ whileR <| b1 | b2 |> do r end }> =>
       LFP (fun (phi : algn_com_dom) =>
              {{ ((stL, stR), (stL', stR')) |
-                ((false, stL) ∈ denote_B b1 /\ stL' = stL /\ stR' = stR)
-                \/ ((false, stR) ∈ denote_B b2 /\ stL' = stL /\ stR' = stR)
-                \/(true, stL) ∈ denote_B b1 /\
+                ((false, stL) ∈ denote_B b1 /\ stL' = RNormal stL /\ stR' = RNormal stR)
+                \/ ((false, stR) ∈ denote_B b2 /\ stL' = RNormal stL /\ stR' = RNormal stR)
+                \/((true, stL) ∈ denote_B b1 /\
+                    (true, stR) ∈ denote_B b2 /\
+                      ((stL, stR), (RError, RError)) ∈ [[r]]R /\
+                        stL' = RError /\ stR' = RError)
+                \/((true, stL) ∈ denote_B b1 /\
                     (true, stR) ∈ denote_B b2 /\
                     exists stL'' stR'',
-                      ((stL, stR), (stL'', stR'')) ∈ [[r]]R /\
-                        ((stL'', stR''), (stL', stR')) ∈ phi }})
+                      ((stL, stR), (RNormal stL'', RNormal stR'')) ∈ [[r]]R /\
+                        ((stL'', stR''), (stL', stR')) ∈ phi) }})
   end
-where "'[[' r ']]R'" := (denote_algn_com r) : denote_scope.
+where "'[[' r ']]R'" := (denote_algn_com r) : denote_scope. *)
+
+
+Fixpoint denote_algn_com (r : algn_com) : algn_com_dom :=
+  match r with
+  | <{ <| s1 | s2 |> }> =>
+      {{ ((stL, stR), (stL', stR')) |
+         (exists st st', (stL, RNormal st) ∈ denote_Com s1 /\ (stR, RNormal st') ∈ denote_Com s2 
+          /\ stL' = RNormal st /\ stR' = RNormal st') }}
+
+  | <{ r1;; r2 }> =>
+      {{ ((stL, stR), (stL', stR')) |
+         (exists stL'' stR'' stL''' stR''',
+         ((stL, stR), (RNormal stL'', RNormal stR'')) ∈ [[ r1 ]]R /\
+           ((stL'', stR''), (RNormal stL''', RNormal stR''')) ∈ [[r2]]R /\ stL' = RNormal stL''' /\ stR' = RNormal stR''') }}
+
+  | <{ ifR <| b1 | b2 |> then r1 else r2 end }> =>
+      {{ ((stL, stR), (stL', stR')) |
+          (exists stL'' stR'', (true, stL) ∈ denote_B b1
+          /\ (true, stR) ∈ (denote_B b2)
+          /\ ((stL, stR), (RNormal stL'', RNormal stR'')) ∈ [[r1]]R /\ stL' = RNormal stL'' /\ stR' = RNormal stR'')
+      \/ (exists stL'' stR'', (false, stL) ∈ (denote_B b1)
+             /\ ((stL, stR), (RNormal stL'', RNormal stR'')) ∈ [[r2]]R /\ stL' = RNormal stL'' /\ stR' = RNormal stR'')
+          \/ (exists stL'' stR'', (false, stR) ∈ (denote_B b2)
+             /\ ((stL, stR), (RNormal stL'', RNormal stR'')) ∈ [[r2]]R /\ stL' = RNormal stL'' /\ stR' = RNormal stR'')}}
+
+(*  rst =<[ r ]>=> (RNormal st, RNormal st') ->
+    (st, st') =<[ whileR <| b1 | b2 |> do r end ]>=> rst' ->
+    rst =<[ whileR <| b1 | b2 |> do r end ]>=> rst'*)
+
+  | <{ whileR <| b1 | b2 |> do r end }> =>
+      LFP (fun (phi : algn_com_dom) =>
+             {{ ((stL, stR), (stL', stR')) |
+                ((false, stL) ∈ denote_B b1 /\ stL' = RNormal stL /\ stR' = RNormal stR)
+                \/ ((false, stR) ∈ denote_B b2 /\ stL' = RNormal stL /\ stR' = RNormal stR)
+                \/((true, stL) ∈ denote_B b1 /\
+                    (true, stR) ∈ denote_B b2 /\
+                    exists stL'' stR'' stL''' stR''',
+                      ((stL, stR), (RNormal stL'', RNormal stR'')) ∈ [[r]]R /\
+                        ((stL'', stR''), (RNormal stL''', RNormal stR''')) ∈ phi /\ stL' = RNormal stL''' /\ stR' = RNormal stR''')}})
+  end
+where "'[[' r ']]R'" := (denote_algn_com r) : denote_scope. 
 
 (* We now show that the two semantics above are equivalent, i.e. that
    our denotational semantics is both sound and adequate with respect
@@ -153,85 +234,121 @@ Lemma while_body_monotone :
     Monotone
       (fun (phi : algn_com_dom) =>
              {{ ((stL, stR), (stL', stR')) |
-                (((false, stL) ∈ denote_B b1 /\ stL' = stL /\ stR' = stR))
-                \/ (((false, stR) ∈ denote_B b2 /\ stL' = stL /\ stR' = stR))
-                \/ (true, stL) ∈ denote_B b1 /\
-                     (true, stR) ∈ denote_B b2 /\
-                     exists stL'' stR'',
-                       ((stL, stR), (stL'', stR'')) ∈ [[r]]R /\
-                         ((stL'', stR''), (stL', stR')) ∈ phi }}).
+                ((false, stL) ∈ denote_B b1 /\ stL' = RNormal stL /\ stR' = RNormal stR)
+                \/ ((false, stR) ∈ denote_B b2 /\ stL' = RNormal stL /\ stR' = RNormal stR)
+                \/((true, stL) ∈ denote_B b1 /\
+                    (true, stR) ∈ denote_B b2 /\
+                    exists stL'' stR'' stL''' stR''',
+                      ((stL, stR), (RNormal stL'', RNormal stR'')) ∈ [[r]]R /\
+                        ((stL'', stR''), (RNormal stL''', RNormal stR''')) ∈ phi /\ stL' = RNormal stL''' /\ stR' = RNormal stR''') }}).
 Proof.
   unfold Monotone, subseteq, set_subseteq_instance, rel_state.
   intros ? ? ? ? ? ? ((st1, st2), (st1', st2')) ?.
   In_inversion; In_intro.
   - firstorder.
   - firstorder.
-  - firstorder.
-Qed.
+  - right. firstorder. simpl in *. right.  firstorder. eexists _,_,_,_.
+    simpl. split. eassumption. split. eapply H. eassumption.
+    firstorder.
+Qed. 
 
 (* Now, soundness: *)
 Lemma BigStep_Denotational_Sound :
-  forall r rst rst',
-    rst =<[r]>=> rst' -> (rst, rst') ∈ [[r]]R.
+  forall r rst st st',
+    rst =<[r]>=> (RNormal st, RNormal st') -> (rst, (RNormal st, RNormal st')) ∈ [[r]]R.
 Proof.
-  intros.
-  induction H;
-    try destruct rst as [stL stR];
+  intros. remember (RNormal st, RNormal st') as re eqn:Heqr.
+  (*remember (rst =<[ r ]>=> (RNormal rst', RNormal rst'')) as re.*)
+  (*rewrite Heqre in H. *)
+    generalize dependent st. revert st'. induction H;
+    try destruct rst as [stL stR]; 
     try destruct rst' as [stL' stR'];
-    try destruct rst'' as [stL'' stR''];
+    (*try destruct rst'' as [stL'' stR''];*)
     simpl in *; try solve [econstructor].
-  - (* EAC_Block *)
-    In_intro; eapply BigStep_Denotational_Sound; eauto.
-  - (* E_ACSeq *)
-    In_intro; eauto.
-  - (* E_ACIfTrue *)
-    left; In_intro; intuition.
-    + rewrite <- H; eapply Denotational_B_BigStep_Sound.
-    + rewrite <- H0; eapply Denotational_B_BigStep_Sound.
-  - (* E_ACIfFalseL *)
-    right; left. intuition.
-    rewrite <- H; eapply Denotational_B_BigStep_Sound.
-  - (* E_ACIfFalseR *)
-    right; right. intuition.
-    rewrite <- H; eapply Denotational_B_BigStep_Sound.
-  - (* E_ACWhileTrue *)
-    apply LFP_unfold.
-    apply while_body_monotone.
-    right; right; intuition.
-    + rewrite <- H; apply Denotational_B_BigStep_Sound.
-    + rewrite <- H0; apply Denotational_B_BigStep_Sound.
-    + eexists _, _; intuition eauto.
-  - (* E_ACWhileFalseL *)
-    apply LFP_unfold; try apply while_body_monotone.
-    left; intuition.
-    rewrite <- H; apply Denotational_B_BigStep_Sound.
-  - (* E_ACWhileFalseR *)
-      apply LFP_unfold; try apply while_body_monotone.
-      right; left. intuition.
-      rewrite <- H; apply Denotational_B_BigStep_Sound.
+  - (* <s1 | s2> none errors *)
+    intros. injection Heqr; intros; subst; clear Heqr. eexists _,_. split.
+    eapply Imp.Semantics.BigStep_Denotational_Sound in H. eassumption.  
+    split. eapply Imp.Semantics.BigStep_Denotational_Sound in H0.
+    eassumption. auto.
+  - (* <s1 | s2|>: s1 Error *)
+     intros. discriminate.
+  -  (*<s1 | s2>: s2 errors*)
+    intros. discriminate.
+  - (*<r1 ;; r2> none error*)
+    intros. inversion Heqr. clear Heqr. subst. eexists _,_,_,_. split.
+    specialize IHaceval1 with st' st. eapply IHaceval1. reflexivity.
+    split. eapply IHaceval2. eauto. eauto.
+  - (* <r1 ;; r2> : r1 error *)
+    intros. discriminate. 
+  - (*If - both true*)
+    intros. inversion Heqr; clear Heqr; subst. left. eexists _,_. firstorder.
+    rewrite <- H. eapply Denotational_B_BigStep_Sound. rewrite <- H0.
+    eapply Denotational_B_BigStep_Sound. specialize IHaceval with st' st.
+    apply IHaceval. reflexivity.
+  - (*If - H b1 false *)
+    intros. right. left. eexists _,_. split. rewrite <- H.
+    eapply Denotational_B_BigStep_Sound. split. specialize IHaceval with st' st.
+    rewrite Heqr in *. eapply IHaceval. reflexivity. inversion Heqr; clear Heqr; subst.
+    eauto.
+  - (*If - H b2 false *)
+    intros. right. right. eexists _,_. split. rewrite <- H. eapply Denotational_B_BigStep_Sound.
+    inversion Heqr; clear Heqr; subst. split. specialize IHaceval with st' st. eapply IHaceval.
+    reflexivity. auto.
+  - (* while - both true and normal *)
+    intros. apply LFP_fold. try apply while_body_monotone. right. right. 
+    split. rewrite <- H. apply Denotational_B_BigStep_Sound.
+    split. rewrite <- H0. apply Denotational_B_BigStep_Sound. 
+    eexists _,_,_,_. split. eapply IHaceval1 with st' st. reflexivity. 
+    split. rewrite Heqr in *. clear Heqr. eapply IHaceval2 with st'0 st0.
+    reflexivity. inversion Heqr; clear Heqr; subst. auto.
+  - (*while error*)
+    intros. discriminate.
+  - (*while b1 is false*) 
+    intros.  apply LFP_unfold. apply while_body_monotone. left.
+    split. rewrite <- H. apply Denotational_B_BigStep_Sound. 
+    inversion Heqr; clear Heqr; subst. auto.
+  - (*while b2 is false*)
+    intros. apply LFP_unfold. apply while_body_monotone. right. left. split.
+    rewrite <- H. apply Denotational_B_BigStep_Sound. auto.
 Qed.
+    
 
 (* Finally, adequacy: *)
 Lemma Denotational_BigStep_Adequate :
-  forall r rst rst',
-    (rst, rst') ∈ [[r]]R -> rst =<[r]>=> rst'.
+  forall r rst st st',
+    (rst, (RNormal st, RNormal st')) ∈ [[r]]R -> rst =<[r]>=> (RNormal st, RNormal st').
 Proof.
   induction r; intros;
     destruct rst as [stL stR];
-    destruct rst' as [stL' stR'];
-    simpl in *; try solve [econstructor]; In_inversion.
-  - econstructor; simpl; eapply Denotational_BigStep_Adequate; eauto.
-  - econstructor; eauto.
-  - eapply E_ACIfTrue; eauto using BigStep_B_Denotational_Adequate; eauto.
-  - eapply E_ACIfFalseL; eauto using BigStep_B_Denotational_Adequate; eauto.
-  - eapply E_ACIfFalseR; eauto using BigStep_B_Denotational_Adequate; eauto.
-  - replace (stL, stR) with (fst ((stL, stR), (stL', stR'))) by reflexivity.
-    replace (stL', stR') with (snd ((stL, stR), (stL', stR'))) by reflexivity.
-    remember (stL, stR, (stL', stR')).
+    simpl in *; try solve [econstructor]; In_inversion. 
+  - (*<s1 | s2>*)
+    simpl in *. inversion H1. inversion H2. econstructor.
+    simpl. eapply Denotational_BigStep_Adequate. assumption.
+    simpl. eapply Denotational_BigStep_Adequate. assumption.
+  - (*<r1 ;; r2>*)
+    simpl in *. inversion H1. inversion H2. econstructor.
+    subst. eapply IHr1. eassumption. subst. eapply IHr2. assumption.
+  - (*if - both true*)
+    simpl in *. eapply E_ACIfTrue. simpl. eapply BigStep_B_Denotational_Adequate.
+    assumption. simpl. eapply BigStep_B_Denotational_Adequate. assumption.
+    specialize IHr1 with (stL, stR) st st'. apply IHr1. inversion H2; subst.
+    inversion H3; subst. assumption.
+  - (*if - b1 false*)
+    simpl in *. eapply E_ACIfFalseL. simpl. eapply BigStep_B_Denotational_Adequate.
+    assumption. specialize IHr2 with (stL, stR) st st'. apply IHr2. 
+    inversion H1; subst. inversion H2; subst. assumption.
+  - (*if - b2 is false*)
+    simpl in *. eapply E_ACIfFalseR. simpl. eapply BigStep_B_Denotational_Adequate.
+    assumption. specialize IHr2 with (stL, stR) st st'. apply IHr2. 
+    inversion H1; subst. inversion H2; subst. assumption.
+  - (*while*)
+    replace (stL, stR) with (fst ((stL, stR), (RNormal st, RNormal st'))) by reflexivity.
+    replace (RNormal st, RNormal st') with (snd ((stL, stR), (RNormal st, RNormal st'))) by reflexivity.
+    remember (stL, stR, (RNormal st, RNormal st')).
     replace (fst (stL, stR, snd p)) with (fst p) by (subst; reflexivity).
     rewrite Heqp.
     revert IHr.
-    pattern (stL, stR, (stL', stR')).
+    pattern (stL, stR, (RNormal st, RNormal st')).
     eapply Ind; try eassumption; clear.
     intros[ [stL stR] [stL' stR'] ] ? ?.
     simpl; In_inversion; intros.
@@ -239,11 +356,11 @@ Proof.
       erewrite BigStep_B_Denotational_Adequate; try reflexivity; assumption.
     + simpl in *; compute in H0, H1; subst. eapply E_ACWhileFalseR.
       erewrite BigStep_B_Denotational_Adequate; try reflexivity; assumption.
-    + eapply E_ACWhileTrue.
+    + eapply E_ACWhileTrueNormal.
       * erewrite BigStep_B_Denotational_Adequate; try reflexivity; assumption.
       * erewrite BigStep_B_Denotational_Adequate; try reflexivity; assumption.
       * apply IHr; eassumption.
-      * simpl in *; eauto.
+      * simpl in *. inversion H3; subst. inversion H4; subst. eauto. 
 Qed.
 
 End Semantics.
